2019-05-29: Merge state and states

src/states/states.v
@@ -4,11 +4,110 @@ Require Import Coq.ZArith.ZArith.
 Require Import Bool.
 
 Require Export util.
+Require Import fun_util.
 Require Export variables.
-Require Export state.
-Require Export functions.
 
 Local Open Scope string_scope.
+
+(* STATE *)
+
+(* VALUE *)
+Inductive VALUE : Type :=
+  | b : bool -> VALUE
+  | i : Z -> VALUE
+  | n : nat -> VALUE.
+  
+Definition eq_value (v1 v2 : VALUE) : Prop :=
+  match v1,v2 with
+  | b t1, b t2 => eq t1 t2
+  | i t1, i t2 => Z.eq t1 t2
+  | n t1, n t2 => t1 = t2
+  | _, _ => False
+  end.
+
+(* STATE *)
+Definition ind_rules_state
+(s : list (NAME * (VALUE * VALUE))) : Prop :=
+  is_function
+    (map (fun var : (NAME * (VALUE * VALUE)) => fst var) s)
+    string_dec.
+
+Record STATE : Set := mkSTATE {
+  state : list (NAME * (VALUE * VALUE))
+  
+  ; rules_state : ind_rules_state state
+}.
+
+Definition previous_values (s : STATE) : list (NAME * VALUE) :=
+  map (fun x => (fst x, (fst (snd x)))) s.(state).
+
+Definition current_values (s : STATE) : list (NAME * VALUE) :=
+  map (fun x => (fst x, (snd (snd x)))) s.(state).
+
+Fixpoint find_var_state
+(n : NAME) (l : list (NAME * (VALUE * VALUE)))
+: option (NAME * (VALUE * VALUE)) :=
+  match l with
+  | []     => None
+  | h :: t => if bstring_dec (fst h) n
+              then Some h else find_var_state n t
+  end.
+
+Definition is_valid_value
+(v : VALUE) (t : TYPE) : Prop :=
+  match v with
+  | b _ => eq_type t Tbool
+  | i _ => eq_type t Tint
+  | n _ => eq_type t Tnat
+  end.
+
+Definition well_typed_var
+(s : STATE) (n : NAME) (t : TYPE) : Prop :=
+  let v := find_var_state n s.(state) in
+    match v with
+    | None   => False
+    | Some p => (is_valid_value (fst (snd p)) t)
+                /\ (is_valid_value (snd (snd p)) t)
+    end.
+
+Fixpoint well_typed_state_var (s:STATE)
+(l: list (NAME * TYPE)) : Prop :=
+    match l with
+    | []     => True
+    | h :: t => well_typed_var s (fst h) (snd h)
+                /\ well_typed_state_var s t
+    end.
+
+Definition well_typed_state (s : STATE)
+(l : list (NAME * TYPE)) : Prop :=
+  let dom_s := map (fun x => fst x) s.(state) in
+  let dom_l := map (fun x => fst x) l in
+    same_list dom_s dom_l string_dec
+    /\ well_typed_state_var s l.
+
+Definition eq_state_element
+(e1 e2 : (NAME * (VALUE * VALUE))) : Prop :=
+  string_dec (fst e1) (fst e2)
+  /\ eq_value (fst (snd e1)) (fst (snd e2))
+  /\ eq_value (snd (snd e1)) (snd (snd e2)).
+
+Fixpoint eq_state_elements (s1 s2 : list (NAME * (VALUE * VALUE))) : Prop :=
+  match s1, s2 with
+  | []      , []       => True
+  | []      , _        => False
+  | _       , []       => False
+  | h1 :: t1, h2 :: t2 => eq_state_element h1 h2
+  end.
+
+Definition eq_state (s1 s2 : STATE) : Prop :=
+  same_list s1.(state) s2.(state) eq_state_element.
+
+(* DFRS_INITIAL_STATE *)
+Record DFRS_INITIAL_STATE : Set := mkDFRS_INITIAL_STATE {
+  s0 : STATE
+}.
+
+(* STATES *)
 
 Definition ind_rules_states (l : list STATE) : Prop :=
   0 < List.length l.
