src/states/states_fun_rules.v
@@ -6,12 +6,80 @@ Require Import Bool.
 Require Export util.
 Require Export fun_util.
 Require Export variables.
-Require Export state.
-Require Export state_fun_rules.
-Require Export functions.
+Require Import variables_fun_rules.
 Require Export states.
 
 Local Open Scope string_scope.
+
+(* STATE *)
+
+(* VALUE *)
+Definition beq_value (v1 v2 : VALUE) : bool :=
+  match v1,v2 with
+  | b t1, b t2 => eqb t1 t2
+  | i t1, i t2 => Z.eqb t1 t2
+  | n t1, n t2 => t1 =? t2
+  | _, _ => false
+  end.
+
+(* STATE *)
+Definition fun_rules_state
+(s : list (NAME * (VALUE * VALUE))) : bool :=
+  bis_function
+    (map (fun var : (NAME * (VALUE * VALUE)) => fst var) s)
+    bstring_dec.
+    
+Definition bis_valid_value
+(v : VALUE) (t : TYPE) : bool :=
+  match v with
+  | b _ => beq_type t Tbool
+  | i _ => beq_type t Tint
+  | n _ => beq_type t Tnat
+  end.
+
+Definition bwell_typed_var
+(s : STATE) (n : NAME) (t : TYPE) : bool :=
+  let v := find_var_state n s.(state) in
+    match v with
+    | None   => false
+    | Some p => (bis_valid_value (fst (snd p)) t)
+                && (bis_valid_value (snd (snd p)) t)
+    end.
+
+Fixpoint bwell_typed_state_var (s:STATE)
+(l: list (NAME * TYPE)) : bool :=
+    match l with
+    | []     => true
+    | h :: t => if bwell_typed_var s (fst h) (snd h)
+                then bwell_typed_state_var s t
+                else false
+    end.
+
+Definition bwell_typed_state (s : STATE)
+(l : list (NAME * TYPE)) : bool :=
+  let dom_s := map (fun x => fst x) s.(state) in
+  let dom_l := map (fun x => fst x) l in
+    bsame_list dom_s dom_l bstring_dec
+    && bwell_typed_state_var s l.
+
+Definition beq_state_element
+(e1 e2 : (NAME * (VALUE * VALUE))) : bool :=
+  bstring_dec (fst e1) (fst e2)
+  && beq_value (fst (snd e1)) (fst (snd e2))
+  && beq_value (snd (snd e1)) (snd (snd e2)).
+
+Fixpoint beq_state_elements (s1 s2 : list (NAME * (VALUE * VALUE))) : bool :=
+  match s1, s2 with
+  | []      , []       => true
+  | []      , _        => false
+  | _       , []       => false
+  | h1 :: t1, h2 :: t2 => beq_state_element h1 h2
+  end.
+
+Definition beq_state (s1 s2 : STATE) : bool :=
+  bsame_list s1.(state) s2.(state) beq_state_element.
+
+(* STATES *)
 
 Definition fun_rules_states (l : list STATE) : bool :=
   0 <? List.length l.
