src/states/states_fun_ind_equiv.v
@@ -1,6 +1,13 @@
 Require Import states.
 Require Import states_fun_rules.
 
+(* STATE *)
+Theorem theo_rules_state :
+  forall (s : list (NAME * (VALUE * VALUE))),
+    ind_rules_state s
+    <-> fun_rules_state s = true.
+Proof. Admitted.
+
 (* STATES *)
 Theorem theo_rules_states :
   forall (ls : list STATE),
