src/trans_rel/trans_rel_fun_rules.v
@@ -7,8 +7,8 @@ Require Export util.
 Require Export fun_util.
 Require Export variables.
 Require Export variables_fun_rules.
-Require Export state.
-Require Export state_fun_rules.
+Require Export states.
+Require Export states_fun_rules.
 Require Export functions.
 Require Export trans_rel.
 
